src/tls/TLSConstants.fst
@@ -1724,30 +1724,3 @@ type serverName =
 type point_format =
   | ECP_UNCOMPRESSED
   | ECP_UNKNOWN of (n:nat{repr_bytes n <= 1})
-
-// deprecated (but still included in TLSInfo)
-type negotiatedExtensions = {
-  ne_extended_ms: bool; // now a total function of the mode
-  ne_extended_padding: bool; // gone!
-  ne_secure_renegotiation: ri_status; // now a total function of the mode
-
-  //$ Cedric: these extensions were missing in F7.
-  ne_server_names: option (list serverName); // now a total function of the mode,
-  ne_keyShare: option CommonDH.serverKeyShare; // now gone (elsewherer in the mode)
-
-  // now internal, transient concerns for server-side nego
-  ne_signature_algorithms: option signatureSchemeList;
-  ne_supported_groups: option (list valid_namedGroup);
-  ne_supported_point_formats: option (list point_format);
-}
-
-let ne_default = {
-  ne_extended_ms = false;
-  ne_extended_padding = false;
-  ne_secure_renegotiation = RI_Unsupported;
-  ne_supported_groups = None;
-  ne_supported_point_formats = None;
-  ne_server_names = None;
-  ne_signature_algorithms = None;
-  ne_keyShare = None;
-}
